checkpoint proving bank with arbitrary list of accounts
left some messy big_sepML-style admits

src/program_proof/memkv/bank_proof.v
@@ -14,6 +14,9 @@ Definition kv_gn γ := γ.(bank_ks_names).
 Definition lk_gn γ := γ.(bank_ls_names).
 Definition log_gn γ := γ.(bank_logBalGN).
 
+Add Ring u64ring : (word.ring_theory (word := u64_instance.u64)).
+
+
 Section bank_defs.
 
 Context `{!invGS Σ, !kvMapG Σ, mapG Σ u64 u64}.
@@ -25,12 +28,10 @@ Definition lockN : namespace := nroot.@"grove_bank_of_boston_vault".
 
 Definition bal_total : u64 := 1000.
 
-Context (init_flag: u64) (acc1:u64) (acc2:u64). (* Account names for bank *)
+Context (init_flag: u64). (* Account names for bank *)
 
 Definition map_total (m : gmap u64 u64) : u64 :=
   map_fold (λ k v tot, word.add tot v) 0 m.
-
-Add Ring u64ring : (word.ring_theory (word := u64_instance.u64)).
 
 Lemma map_total_insert m k v :
   m !! k = None ->
@@ -97,54 +98,51 @@ Definition bank_inv γ (accts : gset u64) : iProp Σ :=
     "%" ∷ ⌜dom m = accts⌝
   .
 
-Definition init_lock_inv γlock γkv : iProp Σ :=
+Definition init_lock_inv γlock γkv accts : iProp Σ :=
   (* Uninit case *)
   (kvptsto γkv init_flag [] ∗
-   kvptsto γkv acc1 [] ∗ kvptsto γkv acc2 [] ∗
-   kvptsto γlock acc1 [] ∗ kvptsto γlock acc2 []
+   [∗ set] acc ∈ accts, kvptsto γkv acc [] ∗ kvptsto γlock acc []
   ) ∨
   (* Already init case *)
   (∃ γlog,
    let γ := {| bank_ls_names := γlock; bank_ks_names := γkv; bank_logBalGN := γlog |} in
-   kvptsto γkv init_flag [U8 0] ∗ inv bankN (bank_inv γ {[acc1; acc2]}) ∗
-   "#Hacc1_is_lock" ∷ is_lock lockN γlock acc1 (bankPs γ acc1) ∗
-   "#Hacc2_is_lock" ∷ is_lock lockN γlock acc2 (bankPs γ acc2)).
+   kvptsto γkv init_flag [U8 0] ∗ inv bankN (bank_inv γ accts) ∗
+    [∗ set] acc ∈ accts, is_lock lockN γlock acc (bankPs γ acc)).
 
 End bank_defs.
 
 Section bank_proof.
 Context `{!heapGS Σ (ext:=grove_op) (ffi:=grove_model), !erpcG Σ, !urpcregG Σ, !kvMapG Σ, mapG Σ u64 u64}.
 
-Context (init_flag: u64) (acc1:u64) (acc2:u64). (* Account names for bank *)
+Context (init_flag: u64). (* Account names for bank *)
 
 
-Definition own_bank_clerk γ (bank_ck:loc) : iProp Σ :=
-  ∃ (lck kck : loc),
-  "%" ∷ ⌜acc1 ≠ acc2⌝ ∗
+Definition own_bank_clerk γ (bank_ck:loc) (accts : gset u64) : iProp Σ :=
+  ∃ (lck kck : loc) (accts_s : Slice.t) (accts_l : list u64),
+  "%" ∷ ⌜Permutation (elements accts) (accts_l)⌝ ∗
   "Hlck_own" ∷ own_LockClerk lck γ.(bank_ls_names) ∗
   "Hkck_own" ∷ own_SeqKVClerk kck γ.(bank_ks_names) ∗
 
   "Hkck" ∷ bank_ck ↦[BankClerk :: "kvck"] #kck ∗
   "Hlck" ∷ bank_ck ↦[BankClerk :: "lck"] #lck ∗
-  "Hacc1" ∷ bank_ck ↦[BankClerk :: "acc1"] #acc1 ∗
-  "Hacc1" ∷ bank_ck ↦[BankClerk :: "acc2"] #acc2 ∗
+  "Haccts" ∷ bank_ck ↦[BankClerk :: "accts"] (slice_val accts_s) ∗
+  "Haccts_slice" ∷ own_slice_small accts_s uint64T 1 accts_l ∗
 
-  "Hacc1_is_lock" ∷ is_lock lockN γ.(bank_ls_names) acc1 (bankPs γ acc1) ∗
-  "Hacc2_is_lock" ∷ is_lock lockN γ.(bank_ls_names) acc2 (bankPs γ acc2)
+  "#Haccts_is_lock" ∷ [∗ list] acc ∈ accts_l, is_lock lockN γ.(bank_ls_names) acc (bankPs γ acc)
 .
 
 
 Lemma acquire_two_spec (lck :loc) (ln1 ln2:u64) γ:
 {{{
      own_LockClerk lck γ.(bank_ls_names) ∗
-     is_lock lockN γ.(bank_ls_names) ln1 (bankPs γ acc1) ∗
-     is_lock lockN γ.(bank_ls_names) ln2 (bankPs γ acc2)
+     is_lock lockN γ.(bank_ls_names) ln1 (bankPs γ ln1) ∗
+     is_lock lockN γ.(bank_ls_names) ln2 (bankPs γ ln2)
 }}}
   acquire_two #lck #ln1 #ln2
 {{{
      RET #(); own_LockClerk lck γ.(bank_ls_names) ∗
-     bankPs γ acc1 ∗
-     bankPs γ acc2
+     bankPs γ ln1 ∗
+     bankPs γ ln2
 }}}.
 Proof.
   iIntros (Φ) "(Hlck & #Hln1_islock & #Hln2_islock) Hpost".
@@ -174,10 +172,10 @@ Qed.
 Lemma release_two_spec (lck :loc) (ln1 ln2:u64) γ:
 {{{
      own_LockClerk lck γ.(bank_ls_names) ∗
-     is_lock lockN γ.(bank_ls_names) ln1 (bankPs γ acc1) ∗
-     is_lock lockN γ.(bank_ls_names) ln2 (bankPs γ acc2) ∗
-     bankPs γ acc1 ∗
-     bankPs γ acc2
+     is_lock lockN γ.(bank_ls_names) ln1 (bankPs γ ln1) ∗
+     is_lock lockN γ.(bank_ls_names) ln2 (bankPs γ ln2) ∗
+     bankPs γ ln1 ∗
+     bankPs γ ln2
 }}}
   release_two #lck #ln1 #ln2
 {{{
@@ -196,29 +194,23 @@ Proof.
   iApply "Hpost"; by iFrame.
 Qed.
 
-Add Ring u64ring : (word.ring_theory (word := u64_instance.u64)).
-
-Lemma Bank__SimpleTransfer_spec (bck:loc) (amount:u64) γ accts :
+Lemma Bank__transfer_internal_spec (bck:loc) src dst (amount:u64) γ accts :
 {{{
      inv bankN (bank_inv γ accts) ∗
-     own_bank_clerk γ bck
+     own_bank_clerk γ bck accts ∗
+     is_lock lockN γ.(bank_ls_names) src (bankPs γ src) ∗
+     is_lock lockN γ.(bank_ls_names) dst (bankPs γ dst) ∗
+     ⌜src ≠ dst⌝
 }}}
-  BankClerk__SimpleTransfer #bck #amount
+  BankClerk__transfer_internal #bck #src #dst #amount
 {{{
      RET #();
-     own_bank_clerk γ bck
+     own_bank_clerk γ bck accts
 }}}.
 Proof.
-  iIntros (Φ) "[#Hbinv Hpre] Hpost".
+  iIntros (Φ) "(#Hbinv & Hpre & #Hsrc & #Hdst & %) Hpost".
   iNamed "Hpre".
-  (* FIXME: iNamed not working correctly? *)
-  iDestruct "Hpre" as "(Hacc1 & Hacc2 & #Hacc_is_lock)".
-  iNamed "Hacc_is_lock".
   wp_lam. wp_pures.
-  wp_loadField.
-  wp_loadField.
-  wp_lam. (* We just use the helper function in-line *)
-  wp_pures.
   wp_loadField.
   wp_apply (acquire_two_spec with "[$Hlck_own]"); first iFrame "#".
   iIntros "(Hlck_own & Hacc1_unlocked & Hacc2_unlocked)".
@@ -273,8 +265,8 @@ Proof.
     iNamed "HbankInv".
     iDestruct (map_valid with "[$] Hacc1_log") as "%Hval1".
     iDestruct (map_valid with "[$] Hacc2_log") as "%Hval2".
-    iMod (map_update acc1 _ (word.sub bal1 amount) with "HlogBalCtx Hacc1_log") as "[HlogBalCtx Hacc1_log]".
-    iMod (map_update acc2 _ (word.add bal2 amount) with "HlogBalCtx Hacc2_log") as "[HlogBalCtx Hacc2_log]".
+    iMod (map_update src _ (word.sub bal1 amount) with "HlogBalCtx Hacc1_log") as "[HlogBalCtx Hacc1_log]".
+    iMod (map_update dst _ (word.add bal2 amount) with "HlogBalCtx Hacc2_log") as "[HlogBalCtx Hacc2_log]".
     iMod ("HbankInvClose" with "[HlogBalCtx]") as "_".
     { iNext. iExists _. iSplitL "HlogBalCtx"; first by iFrame.
       iSplit; iPureIntro.
@@ -290,93 +282,254 @@ Proof.
     { iFrame "#". iSplitL "Hacc1_phys Hacc1_log"; iExists _, _; iFrame; eauto. }
     iIntros "Hlck_own".
     wp_pures. iApply "Hpost".
-    iExists _, _; by iFrame "∗ # %".
+    iExists _, _, _, _; by iFrame "∗ # %".
   - (* Don't do the transfer *)
     wp_loadField. wp_apply (release_two_spec with "[$Hlck_own Hacc1_phys Hacc2_phys Hacc1_log Hacc2_log]").
     { iFrame "#". iSplitL "Hacc1_phys Hacc1_log"; iExists _, _; iFrame; eauto. }
     iIntros "Hlck_own".
     wp_pures. iApply "Hpost".
-    iExists _, _; by iFrame "∗ # %".
+    iExists _, _, _, _; by iFrame "∗ # %".
 Qed.
 
-Lemma Bank__get_total_spec (bck:loc) γ :
+Lemma Bank__SimpleTransfer_spec (bck:loc) γ accts :
 {{{
-     inv bankN (bank_inv γ {[ acc1; acc2 ]}) ∗
-     own_bank_clerk γ bck
+     inv bankN (bank_inv γ accts) ∗
+     own_bank_clerk γ bck accts
+}}}
+  BankClerk__SimpleTransfer #bck
+{{{
+     RET #();
+     own_bank_clerk γ bck accts
+}}}.
+Proof.
+  iIntros (Φ) "[#Hbinv Hpre] Hpost".
+  wp_call.
+  wp_forBreak_cond.
+  wp_pures.
+  wp_apply wp_RandomUint64. iIntros (src) "_".
+  wp_apply wp_RandomUint64. iIntros (dst) "_".
+  wp_apply wp_RandomUint64. iIntros (amount) "_".
+
+  iNamed "Hpre".
+
+  wp_loadField.
+  wp_apply wp_slice_len.
+  wp_pures.
+  destruct (bool_decide (int.Z src < int.Z accts_s.(Slice.sz))) eqn:Hsrc.
+  2: {
+    wp_pures. iModIntro. iLeft. iFrame. iSplit; first by done.
+    iExists _, _, _, _. iFrame "∗%#".
+  }
+
+  wp_loadField.
+  wp_apply wp_slice_len.
+  wp_pures.
+  destruct (bool_decide (int.Z dst < int.Z accts_s.(Slice.sz))) eqn:Hdst.
+  2: {
+    wp_pures. iModIntro. iLeft. iFrame. iSplit; first by done.
+    iExists _, _, _, _. iFrame "∗%#".
+  }
+
+  wp_if_destruct.
+  2: {
+    wp_pures. iModIntro. iLeft. iFrame. iSplit; first by done.
+    iExists _, _, _, _. iFrame "∗%#".
+  }
+
+  iDestruct (slice.own_slice_small_sz with "Haccts_slice") as %Hslicelen.
+  rewrite list_untype_length in Hslicelen.
+
+  destruct (list_lookup_lt _ accts_l (int.nat src)) as (asrc & Hasrc); first by word.
+  destruct (list_lookup_lt _ accts_l (int.nat dst)) as (adst & Hadst); first by word.
+
+  wp_loadField.
+  wp_apply (wp_SliceGet with "[$Haccts_slice]"); first by eauto.
+  iIntros "Haccts_slice".
+
+  wp_loadField.
+  wp_apply (wp_SliceGet with "[$Haccts_slice]"); first by eauto.
+  iIntros "Haccts_slice".
+
+  iDestruct (big_sepL_lookup _ _ _ asrc with "Haccts_is_lock") as "#Hasrc_is_lock"; first by eauto.
+  iDestruct (big_sepL_lookup _ _ _ adst with "Haccts_is_lock") as "#Hadst_is_lock"; first by eauto.
+
+  wp_apply (Bank__transfer_internal_spec with "[-Hpost]").
+  { iFrame "#". iSplitL.
+    - iExists _, _, _, _. iFrame "∗%#".
+    - iPureIntro.
+      intro Hc; subst.
+      assert (NoDup accts_l) as Hnodup.
+      { rewrite -H1. apply NoDup_elements. }
+      epose proof (NoDup_lookup _ _ _ _ Hnodup Hasrc Hadst).
+      apply Heqb. f_equal. f_equal. word.
+  }
+
+  iIntros "Hpre".
+  wp_pures.
+  iModIntro.
+  iLeft.
+  iFrame. done.
+Qed.
+
+Lemma Bank__get_total_spec (bck:loc) γ accts :
+{{{
+     inv bankN (bank_inv γ accts) ∗
+     own_bank_clerk γ bck accts
 }}}
   BankClerk__get_total #bck
 {{{
      RET #bal_total;
-     own_bank_clerk γ bck
+     own_bank_clerk γ bck accts
 }}}.
 Proof.
   iIntros (Φ) "[#Hbinv Hpre] Hpost".
+  wp_call.
+  wp_apply wp_ref_of_zero; first by done.
+  iIntros (sum) "Hsum".
+
   iNamed "Hpre".
-  iDestruct "Hpre" as "(Hacc1 & Hacc2 & #Hacc_is_lock)".
-  iNamed "Hacc_is_lock".
-  wp_lam.
-  repeat wp_loadField.
+  wp_loadField.
+  wp_apply (wp_forSlicePrefix (λ done todo,
+    ∃ locked,
+      "Hlck" ∷ bck ↦[BankClerk :: "lck"] #lck ∗
+      "Hlck_own" ∷ own_LockClerk lck γ.(bank_ls_names) ∗
+      "Hkck" ∷ bck ↦[BankClerk :: "kvck"] #kck ∗
+      "Hkck_own" ∷ own_SeqKVClerk kck γ.(bank_ks_names) ∗
+      "Hsum" ∷ sum ↦[uint64T] #(map_total locked) ∗
+      "Hml" ∷ [∗ maplist] acc ↦ bal;id ∈ locked;done,
+        is_lock lockN γ.(bank_ls_names) acc (bankPs γ acc) ∗
+        ⌜ acc = id ⌝ ∗
+        (∃ (vd : list u8), ⌜has_encoding_Uint64 vd bal⌝ ∗ kvptsto (kv_gn γ) acc vd ∗ acc [[log_gn γ]]↦ bal))%I
+    with "[] [$Haccts_slice Hsum $Hlck $Hlck_own $Hkck $Hkck_own]").
+  2: {
+    iExists ∅. rewrite map_total_empty. iFrame.
+    iApply big_sepML_empty.
+  }
 
-  wp_apply (acquire_two_spec with "[$Hlck_own]"); first iFrame "#".
-  iIntros "(Hlck_own & Hacc1_unlocked & Hacc2_unlocked)".
-  iDestruct "Hacc1_unlocked" as (bd1 bal1) "(%Henc1 & Hacc1_phys & Hacc1_log)".
-  iDestruct "Hacc2_unlocked" as (bd2 bal2) "(%Henc2 & Hacc2_phys & Hacc2_log)".
+  {
+    iIntros (i x done todo) "%".
+    iIntros (Ψ). iModIntro. iIntros "Hpre HΨ".
+    iNamed "Hpre".
 
-  wp_pures.
-  repeat wp_loadField.
-  wp_apply (wp_SeqKVClerk__Get with "[$Hkck_own]").
-  iApply (fupd_mask_intro); first by set_solver. iIntros "Hclo".
-  iExists _. iFrame "Hacc1_phys".
-  iIntros "Hacc1_phys". iMod ("Hclo") as "_". iModIntro.
-  iIntros (v_bal1_g qp1) "(Hkck_own&Hbal1_get)".
-  wp_apply (wp_DecodeUint64' with "[$Hbal1_get //]").
+    wp_loadField.
+    iDestruct (big_sepL_elem_of _ _ x with "Haccts_is_lock") as "#Hx_is_lock".
+    { rewrite -H2. set_solver. }
+    wp_apply (wp_LockClerk__Lock with "[$Hlck_own $Hx_is_lock]").
+    iIntros "[Hlck_own Hx]".
+    iDestruct "Hx" as (x_vd x_bal) "[%Hx_enc [Hx_kv Hx_log]]".
 
-  wp_pures.
-  repeat wp_loadField.
-  wp_apply (wp_SeqKVClerk__Get with "[$Hkck_own]").
-  iApply (fupd_mask_intro); first by set_solver. iIntros "Hclo".
-  iExists _. iFrame "Hacc2_phys".
-  iIntros "Hacc2_phys". iMod ("Hclo") as "_". iModIntro.
-  iIntros (v_bal2_g qp2) "(Hkck_own&Hbal2_get)".
-  wp_apply (wp_DecodeUint64' with "[$Hbal2_get //]").
-  wp_pures.
+    wp_load.
+    wp_loadField.
+    wp_apply (wp_SeqKVClerk__Get with "[$Hkck_own]").
 
+    iApply (fupd_mask_intro); first by set_solver. iIntros "Hclo".
+    iExists _. iFrame "Hx_kv".
+    iIntros "Hx_kv". iMod ("Hclo") as "_". iModIntro.
+    iIntros (v_bal_x_g qp1) "(Hkck_own&Hbal_x_get)".
+    wp_apply (wp_DecodeUint64' with "[$Hbal_x_get //]").
 
-  repeat wp_loadField.
+    wp_pures.
+    wp_store.
+    iModIntro.
+    iApply "HΨ".
+    iExists (<[x := x_bal]> locked).
+    iFrame.
+
+    destruct (decide (x ∈ dom locked)).
+    {
+      apply elem_of_dom in e. destruct e as (?&e).
+      iDestruct (big_sepML_lookup_m_acc _ _ _ _ _ e with "Hml") as (??) "(%He & Hml & _)".
+      iDestruct "Hml" as "(_ & %Heq & _)".
+      subst. exfalso.
+      assert (NoDup (done ++ lv :: todo)) as Hnodup.
+      { rewrite -H1. eapply NoDup_elements. }
+      apply NoDup_app in Hnodup.
+      destruct Hnodup as (_ & Hnodup & _).
+      specialize (Hnodup lv).
+      apply Hnodup; last by econstructor.
+      eapply elem_of_list_lookup_2. eauto.
+    }
+
+    assert (locked !! x = None) as Hnone.
+    { apply not_elem_of_dom_1. eauto. }
+
+    rewrite map_total_insert //.
+    iFrame.
+    iApply big_sepML_insert_app; first by auto.
+    iFrame.
+    iFrame "#".
+    iSplitR; first by done.
+    iExists _. iFrame. done.
+  }
+
+  iIntros "[Haccts_slice Hloop]".
+  iNamed "Hloop".
 
   (* Use inv to know that the sum is total_bal *)
   iApply fupd_wp.
   iInv bankN as ">HbankInv" "HbankInvClose".
   iNamed "HbankInv".
+
+(*
   iDestruct (map_valid with "HlogBalCtx Hacc1_log") as %Hacc1_logphys.
   iDestruct (map_valid with "HlogBalCtx Hacc2_log") as %Hacc2_logphys.
+*)
+  replace (map_total locked) with (map_total m).
+  2: {
+    (* XXX
+     * 1. locked ⊆ m by map_valid for every element in Hml.
+     * 2. dom locked = accts_l (by Hml) = accts (by H1) = dom m (by H3)
+     * 3. thus, locked=m.
+     *)
+    admit.
+  }
+
   iMod ("HbankInvClose" with "[HlogBalCtx]") as "_".
   { iNext. iExists _. iFrame "∗ %". }
   iModIntro.
-  wp_apply (release_two_spec with "[$Hlck_own Hacc1_phys Hacc2_phys Hacc1_log Hacc2_log]"); first iFrame "#".
-  { iSplitL "Hacc1_phys Hacc1_log"; iExists _, _; iFrame; eauto. }
-  iIntros "Hlck_own".
-  wp_pures.
 
-  erewrite (map_total_insert_2 _ acc1) in H2; last by eauto.
-  erewrite (map_total_insert_2 _ acc2) in H2; last by rewrite lookup_delete_ne //.
-  rewrite map_total_dom_empty in H2.
-  2: {
-    rewrite dom_delete_L dom_delete_L H3. set_solver.
+  wp_loadField.
+  wp_apply (wp_forSliceEach
+    ("Hlck" ∷ bck ↦[BankClerk :: "lck"] #lck ∗
+     "Hlck_own" ∷ own_LockClerk lck γ.(bank_ls_names))%I
+    (λ acc,
+     "#Hacc_islock" ∷ is_lock lockN γ.(bank_ls_names) acc (bankPs γ acc) ∗
+     "HbankPs" ∷ bankPs γ acc)%I
+    (λ acc, True)%I
+    with "[] [$Haccts_slice $Hlck $Hlck_own Hml]").
+  {
+    iIntros (?? Ψ) "!> [Hi Hp] HΨ".
+    iNamed "Hi".
+    iNamed "Hp".
+    wp_loadField.
+    wp_apply (wp_LockClerk__Unlock with "[$Hlck_own $Hacc_islock $HbankPs]").
+    iIntros "Hlck_own".
+    iApply "HΨ". iFrame.
   }
-  replace (word.add bal1 bal2) with (bal_total).
-  2: {
-    rewrite -H2 word.add_0_l. ring_simplify. done.
+  {
+    iDestruct (big_sepML_sepL_exists with "Hml") as "Hl".
+    iApply (big_sepL_impl with "Hl").
+    iModIntro. iIntros (??) "%Hsome H".
+    iDestruct "H" as (kk vv) "(%Hlocked & #Hislock & %Heq & HbankPs)".
+    subst.
+    iFrame "Hislock".
+    iDestruct "HbankPs" as (vd) "HbankPs".
+    iExists _, _. iFrame.
   }
 
+  iIntros "[Haccts_slice [Hi Hq]]".
+  iNamed "Hi".
+
+  wp_load.
+  replace (map_total m) with (bal_total) by auto.
   iApply "Hpost".
-  iExists _, _; iFrame "∗ # %"; eauto.
-Qed.
+  iModIntro. iExists _, _, _, _. iFrame "∗#%".
+Admitted.
 
-Lemma Bank__SimpleAudit_spec (bck:loc) γ :
+Lemma Bank__SimpleAudit_spec (bck:loc) γ accts :
 {{{
-     inv bankN (bank_inv γ {[acc1; acc2]}) ∗
-     own_bank_clerk γ bck
+     inv bankN (bank_inv γ accts) ∗
+     own_bank_clerk γ bck accts
 }}}
   BankClerk__SimpleAudit #bck
 {{{
@@ -397,24 +550,26 @@ Proof.
   iModIntro. iLeft. iFrame. eauto.
 Qed.
 
-Lemma wp_MakeBankClerk (lockhost kvhost : u64) cm γ1 γ2 cid  (Hneq: acc1 ≠ acc2) :
+Lemma wp_MakeBankClerk (lockhost kvhost : u64) cm γ1 γ2 cid accts (accts_s : Slice.t) (accts_l : list u64) acc0 :
   {{{
        is_coord_server lockhost γ1 ∗
        is_coord_server kvhost γ2 ∗
        is_ConnMan cm ∗
        is_lock lockN (γ1.(coord_kv_gn)) init_flag
-         (init_lock_inv init_flag acc1 acc2 γ1.(coord_kv_gn) γ2.(coord_kv_gn))
+         (init_lock_inv init_flag γ1.(coord_kv_gn) γ2.(coord_kv_gn) accts) ∗
+       own_slice_small accts_s uint64T 1 accts_l ∗
+       ⌜Permutation (elements accts) accts_l⌝ ∗
+       ⌜accts_l !! int.nat 0 = Some acc0⌝
   }}}
-    MakeBankClerk #lockhost #kvhost #cm #init_flag #acc1 #acc2 #cid
+    MakeBankClerk #lockhost #kvhost #cm #init_flag (slice_val accts_s) #cid
   {{{
-      γ (ck:loc), RET #ck; own_bank_clerk γ ck ∗ inv bankN (bank_inv γ {[acc1; acc2]})
+      γ (ck:loc), RET #ck; own_bank_clerk γ ck accts ∗ inv bankN (bank_inv γ accts)
   }}}
 .
 Proof.
-  iIntros (Φ) "#(Hcoord_lock&Hcoord_kv&#Hcm&Hinit_lock) HΦ".
+  iIntros (Φ) "(#Hcoord_lock&#Hcoord_kv&#Hcm&#Hinit_lock&Haccts_slice&%Hperm&%Hnonempty) HΦ".
   rewrite /MakeBankClerk.
-  wp_lam.
-  wp_pures.
+  wp_call.
   wp_apply wp_allocStruct; first val_ty.
   iIntros (?) "Hl".
   iDestruct (struct_fields_split with "Hl") as "HH".
@@ -426,7 +581,7 @@ Proof.
 
   wp_apply (wp_MakeSeqKVClerk with "[$Hcoord_kv $Hcm]").
   iIntros (kvCk) "Hkv".
-  do 3 wp_storeField.
+  do 2 wp_storeField.
 
   wp_loadField.
   wp_apply (wp_LockClerk__Lock with "[$]").
@@ -438,7 +593,7 @@ Proof.
   wp_loadField.
   wp_apply (wp_SeqKVClerk__Get with "[$Hkv]").
   iDestruct "Hinit" as "[Huninit|Hinit]".
-  - iDestruct "Huninit" as "(Hflag&Hacc1&Hacc2&Hacc_lk1&Hacc_lk2)".
+  - iDestruct "Huninit" as "(Hflag&Haccs)".
     iApply (fupd_mask_weaken ∅); first by set_solver+. iIntros "Hclo'".
     iModIntro. iExists _. iFrame. iIntros "Hflag".
     iMod "Hclo'" as "_". iModIntro.
@@ -449,27 +604,65 @@ Proof.
     iIntros "(Hsl1&Hsl0)".
     wp_pures.
 
-    wp_apply (wp_EncodeUint64).
-    iIntros (??) "(Hacc1_val_slice&%)".
     wp_loadField.
-    iDestruct (own_slice_to_small with "Hacc1_val_slice") as "Hacc1_val_slice".
-    iMod (readonly_alloc_1 with "Hacc1_val_slice") as "#Hacc1_val_Slice".
+    wp_apply (wp_forSliceEach
+      ("kvck" ∷ l ↦[BankClerk :: "kvck"] #kvCk ∗
+       "Hkv" ∷ own_SeqKVClerk kvCk γ2.(coord_kv_gn))%I
+      (λ acc,
+       "Hkv2" ∷ kvptsto γ2.(coord_kv_gn) acc [] ∗
+       "Hkv1" ∷ kvptsto γ1.(coord_kv_gn) acc [])%I
+      (λ acc,
+       ∃ data,
+        kvptsto γ1.(coord_kv_gn) acc [] ∗
+        kvptsto γ2.(coord_kv_gn) acc data ∗
+        ⌜has_encoding_Uint64 data 0⌝)%I with "[] [$Haccts_slice $kvck $Hkv Haccs]").
+    {
+      iIntros (???) "!> [Hi Hp] HΨ".
+      iNamed "Hi".
+      iNamed "Hp".
+      wp_apply (wp_EncodeUint64).
+      iIntros (??) "(Hval_slice&%)".
+      wp_loadField.
+      iDestruct (own_slice_to_small with "Hval_slice") as "Hval_slice".
+      iMod (readonly_alloc_1 with "Hval_slice") as "#Hval_slice".
+      wp_apply (wp_SeqKVClerk__Put with "[$Hkv]"); first by eauto.
+
+      iApply (fupd_mask_intro); first by set_solver. iIntros "Hclo".
+      iExists _. iFrame. iIntros "Hacc1_phys".
+      iMod ("Hclo") as "_". iIntros "!> Hkv".
+      wp_pures.
+
+      iApply "HΨ".
+      iFrame. iExists _. iFrame. done.
+    }
+    {
+      rewrite -Hperm.
+      iApply big_sepS_elements.
+      iApply (big_sepS_impl with "Haccs").
+      iModIntro. iIntros (?) "%Hin [H2 H1]".
+      iFrame.
+    }
+    iIntros "[Haccts_slice [Hi Hq]]".
+    iNamed "Hi".
+
+    wp_apply (wp_EncodeUint64).
+    iIntros (??) "(Hval_slice&%)".
+    wp_loadField.
+    iDestruct (own_slice_to_small with "Hval_slice") as "Hval_slice".
+    iMod (readonly_alloc_1 with "Hval_slice") as "#Hval_slice".
+
+    wp_apply (wp_SliceGet with "[$Haccts_slice]"); first by eauto.
+    iIntros "Haccts_slice".
+    wp_loadField.
     wp_apply (wp_SeqKVClerk__Put with "[$Hkv]"); first by eauto.
+
+    admit.
+(*
     iApply (fupd_mask_intro); first by set_solver. iIntros "Hclo".
     iExists _. iFrame. iIntros "Hacc1_phys".
     iMod ("Hclo") as "_". iIntros "!> Hkv".
     wp_pures.
-
-    wp_apply (wp_EncodeUint64).
-    iIntros (??) "(Hacc2_val_slice&%)".
-    wp_loadField.
-    iDestruct (own_slice_to_small with "Hacc2_val_slice") as "Hacc2_val_slice".
-    iMod (readonly_alloc_1 with "Hacc2_val_slice") as "#Hacc2_val_Slice".
-    wp_apply (wp_SeqKVClerk__Put with "[$Hkv]"); first by eauto.
-    iApply (fupd_mask_intro); first by set_solver. iIntros "Hclo".
-    iExists _. iFrame. iIntros "Hacc2_phys".
-    iMod ("Hclo") as "_". iIntros "!> Hkv".
-    wp_pures.
+  
 
     wp_apply (typed_slice.wp_NewSlice (V:=u8)).
     iIntros (?) "Hflag_val_slice".
@@ -508,7 +701,8 @@ Proof.
     { iRight. iExists γlog. iFrame "#". iFrame "Hflag_phys". }
     iIntros "H". wp_pures. iApply "HΦ". iModIntro. iFrame "Hinv".
     iExists _, _. iFrame. eauto.
-  - iDestruct "Hinit" as (γlog) "(Hflag&#Hinv&H)". iNamed "H".
+*)
+  - iDestruct "Hinit" as (γlog) "(Hflag&#Hinv&#H)".
     iApply (fupd_mask_weaken ∅); first by set_solver+. iIntros "Hclo'".
     iModIntro. iExists _. iFrame. iIntros "Hflag".
     iMod "Hclo'" as "_". iModIntro.
@@ -520,10 +714,10 @@ Proof.
     wp_pures.
     wp_loadField.
     wp_apply (wp_LockClerk__Unlock with "[$Hlk $Hinit_lock Hflag]").
-    { iRight. iExists γlog. iFrame "#". eauto. }
-    iIntros "H". wp_pures. iApply "HΦ". iModIntro. iFrame "Hinv".
-    iExists _, _. iFrame. eauto.
-Qed.
+    { iRight. iExists γlog. iFrame "∗#". }
+    iIntros "Hlck_own". wp_pures. iApply "HΦ". iModIntro. iFrame "Hinv".
+    iExists _, _, _, _. iFrame "∗#%".
+    iDestruct (big_sepS_elements with "H") as "He". rewrite Hperm. iFrame "He".
+Admitted.
 
 End bank_proof.
-
